theories/iris/logrel/instr/typing/unfold.v
@@ -50,7 +50,7 @@ Section unfold.
       destruct Hmono as [ρ [Hrep _]].
       inversion Hrep as [? ? ? ? Hhas_kind]; subst.
       inversion Hhas_kind; subst.
-      constructor. assumption.
+      econstructor; eauto.
     }
     unfold τrec.
 
@@ -70,7 +70,10 @@ Section unfold.
     Transparent senv_insert_type.
     iModIntro.
     inversion Hkind; subst.
-    assert (Hkindτrec: has_kind F τrec κ) by by apply has_kind_rec_subst.
+    assert (∃ κrec, subkind_of κrec κ ∧ has_kind F τrec κrec)
+      as (κrec & Hsub & Hkindτrec)
+      by by apply has_kind_rec_subst.
+
     destruct (refresh_kinds_id) as (this & _).
     assert (refresh_kinds F τrec = τrec) by (symmetry; by eapply this).
     unfold τrec in H0.
